According to the SNAME(1950) it is standard to express the submerged weight of the body and buoyance force as:

$$
W = mg
$$
$$
B = \rho g\nabla
$$
$\rho$ = water density
$\nabla$ = volume of fluid displaced by the vehicle
m = mass of the vessel including water in free flooding space
g = acceleration of gravity

![[u_boat.png]]

Gravitational force on vector form:
$$
f^n_{g} = \begin{bmatrix}
0 \\
0 \\
W
\end{bmatrix}
$$
Buoyancy force on vector form:
$$
f^n_{b} = -\begin{bmatrix}
0 \\
0 \\
B
\end{bmatrix}
$$
These forces can be transformed from **NED** to **BODY** by the following transformation:
$$
f^b_{g} = R^T(\Theta_{nb})f^n_{g}
$$
$$
f^b_{b} = R^T(\Theta_{nb})f^n_{b}
$$
#### Generalized restoring force in BODY with coordinate origin CO
$$
g(\eta) = \begin{bmatrix}
f^b_{g}+f^b_{b} \\
r^b_{bg}\times f^b_{g}+r^b_{bb}\times f^b_{b} 
\end{bmatrix}
$$
where 
$$
r^b_{bg} := \begin{bmatrix}
x_{g},y_{g},z_{g}
\end{bmatrix}^T
$$
$$
r^b_{bb} := \begin{bmatrix}
x_{b},y_{b},z_{b}
\end{bmatrix}^T
$$

center of buoyance with respect to the CO
center of gravity with respect to the CO

Multiplying out the generalized restoring force we get:
$$
g(\eta)=\begin{bmatrix}
(W-B)\sin \theta \\
-(W-B)\cos \theta \sin \phi \\
-(W-B)\cos \theta \cos \phi \\
-(y_{g}W-y_{b}B)\cos \theta \cos \phi+(z_{g}W-z_{b}B)\cos \theta \sin \phi \\
(z_{g}W-z_{b}B\sin \theta)+(x_{g}W-x_{b}B)\cos \theta \cos \phi \\
-(x_{g}W-x_{b}B)\cos \theta \sin \phi-(y_{g}W-y_{b}B)\sin \theta
\end{bmatrix}
$$
It is possible to simplify this matrix by assuming the underwater vehicle is **neutrally buoyant** W=B:
$$
g(\eta)=\begin{bmatrix}
0 \\
0 \\
0 \\
-BG_{y}W\cos \theta \cos \phi+BG_{z}W\cos \theta \sin \phi \\
BG_{z}W\sin \theta+BG_{x}W\cos \theta \cos \phi \\
-BG_{x}W\cos \theta \sin \phi-BG_{y}W\sin \theta
\end{bmatrix}
$$
An even simpler representation is obtained for vehicles where CG and CB are located vertically on the z-axis, that is $x_{b}= x_{g}$ and $y_{g} = y_{b}$
$$
g(\eta) = \begin{bmatrix}
0 & 0 & 0 & BG_{z}W\cos \theta \sin \phi & BG_{z}W\sin \theta & 0
\end{bmatrix}^T
$$


